include/s2n-bignum-c89.h
@@ -977,8 +977,8 @@ extern void edwards25519_scalarmuldouble_alt(uint64_t res[8],uint64_t scalar[4],
 extern void mlkem_intt(int16_t a[256],int16_t z_01234[80],int16_t z_56[384]);
 
 /* Keccak-f1600 permutation for SHA3 */
-/* Input a[25]; output a[25] */
-extern void mlkem_keccak_f1600(uint64_t a[25]);
+/* Inputs a[25], rc[24]; output a[25] */
+extern void mlkem_keccak_f1600(uint64_t a[25],uint64_t rc[24]);
 
 /* Forward number-theoretic transform from ML-KEM */
 /* Input a[256] (signed 16-bit words), z_01234[80] (signed 16-bit words), z_56[384] (signed 16-bit words); output a[256] (signed 16-bit words) */
